ZhukLean.lean
@@ -2,6 +2,7 @@ import ZhukLean.Product
 import ZhukLean.Absorption
 import ZhukLean.StarPower
 import ZhukLean.Essential
+import ZhukLean.Regrouping
 import ZhukLean.Center
 import ZhukLean.Step
 import ZhukLean.Absorbs
